WIP

security/Backtranslation.v
@@ -181,6 +181,8 @@ Section Backtranslation.
   Section CODE.
     (** converting trace to code **)
 
+    Definition wf_env (e: env) id := e ! id = None.
+
     Definition eventval_to_type (v: eventval): type :=
       match v with
       | EVint _ => Tint I32 Signed noattr
@@ -205,7 +207,7 @@ Section Backtranslation.
 
     Lemma ptr_of_id_ofs_eval
           id ofs e (ge: genv) b cp le m
-          (GE1: e ! id = None)
+          (GE1: wf_env e id)
           (GE2: Genv.find_symbol ge id = Some b)
       :
       eval_expr ge e cp le m (ptr_of_id_ofs id ofs) (Vptr b ofs).
@@ -236,40 +238,35 @@ Section Backtranslation.
       | EVptr_global id ofs => ptr_of_id_ofs id ofs
       end.
 
-    Definition wf_eventval (ge: genv) (e: env) (v: eventval): Prop :=
+    Definition wf_eventval_env (e: env) (v: eventval): Prop :=
       match v with
-      | EVptr_global id _ => (e ! id = None) /\ (Senv.public_symbol ge id = true)
+      | EVptr_global id _ => wf_env e id
       | _ => True
       end.
 
-    Definition wf_eventval_weak (ge: genv) (e: env) (v: eventval): Prop :=
+    Definition wf_eventval_pub (ge: genv) (v: eventval): Prop :=
       match v with
-      | EVptr_global id _ => (e ! id = None) /\ (exists b, Genv.find_symbol ge id = Some b)
+      | EVptr_global id _ => (Senv.public_symbol ge id = true)
       | _ => True
       end.
 
-    Lemma wf_eventval_weak_weak
-          ge e v
-      :
-      wf_eventval ge e v -> wf_eventval_weak ge e v.
-    Proof. intros H. destruct v; simpl in *; auto. destruct H. split; auto. apply Genv.public_symbol_exists in H0. auto. Qed.
-
-    Definition wf_eventval_weak2 (ge: genv) (v: eventval): Prop :=
+    Definition wf_eventval_ge (ge: genv) (v: eventval): Prop :=
       match v with
       | EVptr_global id _ => (exists b, Genv.find_symbol ge id = Some b)
       | _ => True
       end.
 
-    Lemma wf_eventval_weak2_weak
-          ge e v
+    Lemma wf_eventval_pub_ge
+          ge v
       :
-      wf_eventval_weak ge e v -> wf_eventval_weak2 ge v.
-    Proof. intros H. destruct v; simpl in *; auto. destruct H. auto. Qed.
+      wf_eventval_pub ge v -> wf_eventval_ge ge v.
+    Proof. intros H. destruct v; simpl in *; auto. apply Genv.public_symbol_exists in H; auto. Qed.
 
     Lemma eventval_to_expr_match
           ge env cp le m
           ev exp v ty
-          (WFEV: wf_eventval ge env ev)
+          (WFENV: wf_eventval_env env ev)
+          (WFGE: wf_eventval_pub ge ev)
           (CONV: eventval_to_expr ev = exp)
           (EVAL: eval_expr ge env cp le m exp v)
           (TYPE: typ_of_type (eventval_to_type ev) = ty)
@@ -281,7 +278,7 @@ Section Backtranslation.
       - inversion EVAL; subst; simpl in *; try constructor. inversion H.
       - inversion EVAL; subst; simpl in *; try constructor. inversion H.
       - inversion EVAL; subst; simpl in *; try constructor. inversion H.
-      - destruct WFEV as [WFEV1 WFEV2]. unfold ptr_of_id_ofs in EVAL. destruct Archi.ptr64 eqn:ARCH.
+      - unfold ptr_of_id_ofs in EVAL. destruct Archi.ptr64 eqn:ARCH.
         + inversion EVAL; subst; simpl in *; try constructor.
           2:{ inversion H. }
           inversion H5; subst; simpl in *.
@@ -289,7 +286,7 @@ Section Backtranslation.
           clear H5. inversion H4; subst; simpl in *.
           2:{ inversion H. }
           clear H4. inversion H2; subst; simpl.
-          { rewrite WFEV1 in H4. inversion H4. }
+          { rewrite WFENV in H4. inversion H4. }
           { inversion H6.
             rewrite Ptrofs.mul_commut, Ptrofs.mul_one.
             rewrite Ptrofs.add_zero_l.
@@ -304,7 +301,7 @@ Section Backtranslation.
           clear H5. inversion H4; subst; simpl in *.
           2:{ inversion H. }
           clear H4. inversion H2; subst; simpl.
-          { rewrite WFEV1 in H4. inversion H4. }
+          { rewrite WFENV in H4. inversion H4. }
           { inversion H6.
             rewrite Ptrofs.mul_commut, Ptrofs.mul_one.
             rewrite Ptrofs.add_zero_l.
@@ -341,13 +338,14 @@ Section Backtranslation.
 
     Lemma eventval_to_expr_val_eval
           ge en cp temp m ev
-          (WF: wf_eventval_weak ge en ev)
+          (WFENV: wf_eventval_env en ev)
+          (WFGE: wf_eventval_ge ge ev)
       :
       eval_expr ge en cp temp m (eventval_to_expr ev) (eventval_to_val ge ev).
     Proof.
       destruct ev; simpl in *; try constructor.
-      destruct WF as [WF0 [b WF1]].
-      rewrite WF1. unfold ptr_of_id_ofs. destruct Archi.ptr64 eqn:ARCH.
+      destruct WFGE as [b WFGE].
+      rewrite WFGE. unfold ptr_of_id_ofs. destruct Archi.ptr64 eqn:ARCH.
       - econstructor; try econstructor. eapply eval_Evar_global; eauto.
         simpl. simpl_expr. rewrite Ptrofs.mul_commut, Ptrofs.mul_one. rewrite Ptrofs.add_zero_l.
         rewrite Ptrofs.of_int64_to_int64; auto.
@@ -359,14 +357,15 @@ Section Backtranslation.
     Lemma eventval_to_expr_val_match
           ge env
           ev exp v ty
-          (WFEV: wf_eventval ge env ev)
+          (WFENV: wf_eventval_env env ev)
+          (WFEV: wf_eventval_pub ge ev)
           (CONV0: eventval_to_expr ev = exp)
           (CONV1: eventval_to_val ge ev = v)
           (TYPE: typ_of_type (eventval_to_type ev) = ty)
       :
       eventval_match ge ev ty v.
     Proof.
-      subst. eapply eventval_to_expr_match; eauto. eapply eventval_to_expr_val_eval; eauto. apply wf_eventval_weak_weak; auto.
+      subst. eapply eventval_to_expr_match; eauto. eapply eventval_to_expr_val_eval; eauto. apply wf_eventval_pub_ge; auto.
       Unshelve. exact default_compartment. exact (PTree.empty val). exact Mem.empty.
     Qed.
 
@@ -378,34 +377,40 @@ Section Backtranslation.
 
     Lemma sem_cast_eventval
           ge v m
-          (WFEV: wf_eventval_weak2 ge v)
+          (WFEV: wf_eventval_ge ge v)
       :
       Cop.sem_cast (eventval_to_val ge v) (typeof (eventval_to_expr v)) (eventval_to_type v) m = Some (eventval_to_val ge v).
     Proof. rewrite typeof_eventval_to_expr_type. destruct v; simpl in *; simpl_expr. destruct WFEV. rewrite H. simpl_expr. Qed.
 
     Lemma list_eventval_to_expr_val_eval
           ge en cp temp m evs
-          (WF: Forall (wf_eventval_weak ge en) evs)
+          (WFENV: Forall (wf_eventval_env en) evs)
+          (WFGE: Forall (wf_eventval_ge ge) evs)
       :
       eval_exprlist ge en cp temp m (list_eventval_to_list_expr evs) (list_eventval_to_typelist evs) (list_eventval_to_list_val ge evs).
     Proof.
-      move evs at top. revert ge en cp temp m WF. induction evs; intros; simpl in *. constructor.
-      inversion WF; clear WF; subst. econstructor; eauto. eapply eventval_to_expr_val_eval; eauto.
-      apply sem_cast_eventval. eapply wf_eventval_weak2_weak; eauto.
+      move evs at top. revert ge en cp temp m WFENV WFGE. induction evs; intros; simpl in *.
+      constructor.
+      inversion WFENV; clear WFENV; subst. inversion WFGE; clear WFGE; subst.
+      econstructor; eauto. eapply eventval_to_expr_val_eval; eauto.
+      apply sem_cast_eventval; auto.
     Qed.
 
     Lemma list_eventval_to_expr_val_match
           ge env
           evs exps vs tys
-          (WFEV: Forall (wf_eventval ge env) evs)
+          (WFENV: Forall (wf_eventval_env env) evs)
+          (WFPUB: Forall (wf_eventval_pub ge) evs)
           (CONV0: list_eventval_to_list_expr evs = exps)
           (CONV1: list_eventval_to_list_val ge evs = vs)
           (TYPE: list_eventval_to_typelist evs = tys)
       :
       eventval_list_match ge evs (typlist_of_typelist tys) vs.
     Proof.
-      move evs at top. revert ge env exps vs tys WFEV CONV0 CONV1 TYPE. induction evs; intros; simpl in *; subst. constructor.
-      inversion WFEV; clear WFEV; subst. econstructor; eauto. eapply eventval_to_expr_val_match; eauto.
+      move evs at top. revert ge env exps vs tys WFENV WFPUB CONV0 CONV1 TYPE.
+      induction evs; intros; simpl in *; subst. constructor.
+      inversion WFENV; clear WFENV; subst. inversion WFPUB; clear WFPUB; subst.
+      econstructor; eauto. eapply eventval_to_expr_val_match; eauto.
     Qed.
 
 
@@ -455,7 +460,7 @@ Section Backtranslation.
           p f k e le m
           (EV: ev = Event_vload ch id ofs v)
           (* bt should ensure them *)
-          (GLOB: e ! id = None)
+          (WFENV: wf_env e id)
           b
           (VOL: Senv.block_is_volatile (globalenv p) b = true)
           (GE: Genv.find_symbol (globalenv p) id = Some b)
@@ -498,12 +503,13 @@ Section Backtranslation.
           p f k e le m
           (EV: ev = Event_vstore ch id ofs v)
           (* bt should ensure them *)
-          (GLOB: e ! id = None)
+          (WFENV: wf_env e id)
           b
           (VOL: Senv.block_is_volatile (globalenv p) b = true)
           (GE: Genv.find_symbol (globalenv p) id = Some b)
           (* asm should ensure them *)
-          (WFSV: wf_eventval_weak (globalenv p) e v)
+          (WFSV1: wf_eventval_env e v)
+          (WFSV2: wf_eventval_ge (globalenv p) v)
           (MATCH: eventval_match (globalenv p) v (type_of_chunk ch) (Val.load_result ch (eventval_to_val (globalenv p) v)))
       :
         Star (Clight.semantics1 p)
@@ -520,8 +526,8 @@ Section Backtranslation.
             { eapply ptr_of_id_ofs_eval; eauto. }
             { unfold ptr_of_id_ofs; simpl. rewrite ARCH. simpl. simpl_expr. }
             econstructor; eauto. 3: econstructor.
-            { eapply eventval_to_expr_val_eval. auto. }
-            { apply sem_cast_eventval. eapply wf_eventval_weak2_weak; eauto. }
+            { eapply eventval_to_expr_val_eval; auto. }
+            { apply sem_cast_eventval; auto. }
           }
           simpl.
           repeat econstructor; eauto.
@@ -534,8 +540,8 @@ Section Backtranslation.
             { eapply ptr_of_id_ofs_eval; eauto. }
             { unfold ptr_of_id_ofs; simpl. rewrite ARCH. simpl. simpl_expr. }
             econstructor; eauto. 3: econstructor.
-            { eapply eventval_to_expr_val_eval. auto. }
-            { apply sem_cast_eventval. eapply wf_eventval_weak2_weak; eauto. }
+            { eapply eventval_to_expr_val_eval; auto. }
+            { apply sem_cast_eventval; auto. }
           }
           simpl.
           repeat econstructor; eauto.
@@ -549,7 +555,8 @@ Section Backtranslation.
           p f k e le m
           (EV: ev = Event_annot str vs)
           (* bt should ensure them *)
-          (WF: Forall (wf_eventval (globalenv p) e) vs)
+          (WFENV: Forall (wf_eventval_env e) vs)
+          (WFPUB: Forall (wf_eventval_pub (globalenv p)) vs)
           (* asm should ensure them *)
       :
         Star (Clight.semantics1 p)
@@ -561,7 +568,8 @@ Section Backtranslation.
       econstructor 2.
       3:{ rewrite E0_right. reflexivity. }
       { eapply step_builtin.
-        { eapply list_eventval_to_expr_val_eval. eapply Forall_impl. 2: eauto. intros. apply wf_eventval_weak_weak; auto. }
+        { eapply list_eventval_to_expr_val_eval; auto.
+          eapply Forall_impl. 2: eauto. intros. apply wf_eventval_pub_ge; auto. }
         repeat econstructor; eauto. eapply list_eventval_to_expr_val_match; eauto.
       }
       econstructor 1.
@@ -581,7 +589,8 @@ Section Backtranslation.
           fd
           (FINDF: Genv.find_funct ge (Vptr b Ptrofs.zero) = Some fd)
           (TYPEF: type_of_fundef fd = Tfunction (list_eventval_to_typelist vs) Tvoid cc_default)
-          (WFARGS: Forall (wf_eventval ge e) vs)
+          (WFARGS1: Forall (wf_eventval_env e) vs)
+          (WFARGS2: Forall (wf_eventval_pub ge) vs)
           (* asm should ensure them *)
           (CP1: cp = comp_of f)
           (CP2: cp' = comp_of fd)
@@ -602,7 +611,8 @@ Section Backtranslation.
           - eapply eval_Evar_global; eauto.
           - eapply deref_loc_reference. auto.
         }
-        { eapply list_eventval_to_expr_val_eval. eapply Forall_impl. 2: eauto. intros. apply wf_eventval_weak_weak; auto. }
+        { eapply list_eventval_to_expr_val_eval; auto.
+          eapply Forall_impl. 2: eauto. intros. apply wf_eventval_pub_ge; auto. }
         red; auto.
         unfold Genv.find_comp. setoid_rewrite FINDF.
         eapply call_trace_cross; eauto. apply Genv.find_invert_symbol; auto.
@@ -670,7 +680,8 @@ Section Backtranslation.
           (GE: ge = globalenv p)
           (EV: ev = Event_return cp' cp rv)
           (* bt should ensure them *)
-          (WFRV: wf_eventval ge e rv)
+          (WFRV1: wf_eventval_env e rv)
+          (WFRV2: wf_eventval_pub ge rv)
           (RTTYP: fn_return f = eventval_to_type rv)
           (* asm should ensure them *)
           optid f' e' le' k'
@@ -692,9 +703,8 @@ Section Backtranslation.
       econstructor 2.
       3:{ rewrite E0_left. reflexivity. }
       { eapply step_return_1; simpl; eauto.
-        { eapply eventval_to_expr_val_eval; auto. apply wf_eventval_weak_weak; auto. }
-        { rewrite RTTYP. eapply sem_cast_eventval.
-          eapply wf_eventval_weak2_weak. eapply wf_eventval_weak_weak; eauto. }
+        { eapply eventval_to_expr_val_eval; auto. apply wf_eventval_pub_ge; auto. }
+        { rewrite RTTYP. eapply sem_cast_eventval; auto. eapply wf_eventval_pub_ge; eauto. }
       }
       econstructor 2.
       3:{ rewrite E0_right. reflexivity. }
@@ -705,32 +715,16 @@ Section Backtranslation.
       econstructor 1.
     Qed.
 
-    (* TODO *)
-
   End CODE.
 
 
   Section PROJ.
     (** Projection of the trace according to compartments **)
 
-    (* Definition curr_comp_of_event (e: event): option compartment := *)
-    (*   match e with *)
-    (*   | Event_call cp cp' id vs => Some cp *)
-    (*   | Event_return cp cp' v => Some cp' *)
-    (*   | _ => None *)
-    (*   end. *)
-
-    (* Definition next_comp_of_event (e: event): option compartment := *)
-    (*   match e with *)
-    (*   | Event_call cp cp' id vs => Some cp' *)
-    (*   | Event_return cp cp' v => Some cp *)
-    (*   | _ => None *)
-    (*   end. *)
-
     Definition comp_of_event (e: event): option (compartment * compartment) :=
       match e with
       | Event_call cp cp' id vs => Some (cp, cp')
-      | Event_return cp cp' v => Some (cp', cp)
+      | Event_return cp' cp v => Some (cp, cp')
       | _ => None
       end.
 
@@ -757,6 +751,286 @@ Section Backtranslation.
       map fst (PTree.elements p.(Policy.policy_export)).
 
   End PROJ.
+
+
+  Section WELLFORMED.
+
+    Variable p: program.
+    Let ge := globalenv p.
+
+    (** Well-formed conditions for the trace, namely from the semantics of Asm **)
+    Definition wf_trace_vload ch v :=
+      exists rv, eventval_match (globalenv p) v (type_of_chunk ch) rv.
+
+
+    (** Well-formed conditions for the back-translated program **)
+    Definition wf_bt_vload (e: env) id :=
+      (wf_env e id) /\
+        (exists b, (Genv.find_symbol ge id = Some b) /\ (Senv.block_is_volatile ge b = true)).
+      
+
+    Lemma code_of_event_step_vload
+          ev
+          ch id ofs v
+          p f k e le m
+          (EV: ev = Event_vload ch id ofs v)
+          (* bt should ensure them *)
+          (WFENV: wf_env e id)
+          b
+          (VOL: Senv.block_is_volatile (globalenv p) b = true)
+          (GE: Genv.find_symbol (globalenv p) id = Some b)
+          (* asm should ensure them *)
+          rv
+          (MATCH: eventval_match (globalenv p) v (type_of_chunk ch) rv)
+      :
+        Star (Clight.semantics1 p)
+             (State f (code_of_event ev) k e le m)
+             (ev :: nil)
+             (State f Sskip k e le m).
+    Proof.
+      subst; simpl in *. unfold code_of_vload.
+      destruct Archi.ptr64 eqn:ARCH.
+      - econstructor 2.
+        3:{ rewrite E0_right. reflexivity. }
+        { eapply step_builtin.
+          { econstructor; eauto. 3: econstructor.
+            - eapply ptr_of_id_ofs_eval; eauto.
+            - unfold ptr_of_id_ofs; simpl. rewrite ARCH. simpl. simpl_expr.
+          }
+          repeat econstructor; eauto.
+        }
+        econstructor 1.
+      - econstructor 2.
+        3:{ rewrite E0_right. reflexivity. }
+        { eapply step_builtin.
+          { econstructor; eauto. 3: econstructor.
+            - eapply ptr_of_id_ofs_eval; eauto.
+            - unfold ptr_of_id_ofs; simpl. rewrite ARCH. simpl. simpl_expr.
+          }
+          repeat econstructor; eauto.
+        }
+        econstructor 1.
+    Qed.
+
+    Lemma code_of_event_step_vstore
+          ev
+          ch id ofs v
+          p f k e le m
+          (EV: ev = Event_vstore ch id ofs v)
+          (* bt should ensure them *)
+          (WFENV: wf_env e id)
+          b
+          (VOL: Senv.block_is_volatile (globalenv p) b = true)
+          (GE: Genv.find_symbol (globalenv p) id = Some b)
+          (* asm should ensure them *)
+          (WFSV1: wf_eventval_env e v)
+          (WFSV2: wf_eventval_ge (globalenv p) v)
+          (MATCH: eventval_match (globalenv p) v (type_of_chunk ch) (Val.load_result ch (eventval_to_val (globalenv p) v)))
+      :
+        Star (Clight.semantics1 p)
+             (State f (code_of_event ev) k e le m)
+             (ev :: nil)
+             (State f Sskip k e le m).
+    Proof.
+      subst; simpl in *. unfold code_of_vstore.
+      destruct Archi.ptr64 eqn:ARCH.
+      - econstructor 2.
+        3:{ rewrite E0_right. reflexivity. }
+        { eapply step_builtin.
+          { econstructor; eauto.
+            { eapply ptr_of_id_ofs_eval; eauto. }
+            { unfold ptr_of_id_ofs; simpl. rewrite ARCH. simpl. simpl_expr. }
+            econstructor; eauto. 3: econstructor.
+            { eapply eventval_to_expr_val_eval; auto. }
+            { apply sem_cast_eventval; auto. }
+          }
+          simpl.
+          repeat econstructor; eauto.
+        }
+        econstructor 1.
+      - econstructor 2.
+        3:{ rewrite E0_right. reflexivity. }
+        { eapply step_builtin.
+          { econstructor; eauto.
+            { eapply ptr_of_id_ofs_eval; eauto. }
+            { unfold ptr_of_id_ofs; simpl. rewrite ARCH. simpl. simpl_expr. }
+            econstructor; eauto. 3: econstructor.
+            { eapply eventval_to_expr_val_eval; auto. }
+            { apply sem_cast_eventval; auto. }
+          }
+          simpl.
+          repeat econstructor; eauto.
+        }
+        econstructor 1.
+    Qed.
+
+    Lemma code_of_event_step_annot
+          ev
+          str vs
+          p f k e le m
+          (EV: ev = Event_annot str vs)
+          (* bt should ensure them *)
+          (WFENV: Forall (wf_eventval_env e) vs)
+          (WFPUB: Forall (wf_eventval_pub (globalenv p)) vs)
+          (* asm should ensure them *)
+      :
+        Star (Clight.semantics1 p)
+             (State f (code_of_event ev) k e le m)
+             (ev :: nil)
+             (State f Sskip k e le m).
+    Proof.
+      subst; simpl in *. unfold code_of_annot.
+      econstructor 2.
+      3:{ rewrite E0_right. reflexivity. }
+      { eapply step_builtin.
+        { eapply list_eventval_to_expr_val_eval; auto.
+          eapply Forall_impl. 2: eauto. intros. apply wf_eventval_pub_ge; auto. }
+        repeat econstructor; eauto. eapply list_eventval_to_expr_val_match; eauto.
+      }
+      econstructor 1.
+    Qed.
+
+    Lemma code_of_event_step_call_start
+          ev
+          cp cp' id vs
+          p f k e le m
+          ge
+          (GE: ge = globalenv p)
+          (EV: ev = Event_call cp cp' id vs)
+          (* bt should ensure them *)
+          (GLOB: e ! id = None)
+          b
+          (FINDB: Genv.find_symbol ge id = Some b)
+          fd
+          (FINDF: Genv.find_funct ge (Vptr b Ptrofs.zero) = Some fd)
+          (TYPEF: type_of_fundef fd = Tfunction (list_eventval_to_typelist vs) Tvoid cc_default)
+          (WFARGS1: Forall (wf_eventval_env e) vs)
+          (WFARGS2: Forall (wf_eventval_pub ge) vs)
+          (* asm should ensure them *)
+          (CP1: cp = comp_of f)
+          (CP2: cp' = comp_of fd)
+          (NPTR: Forall not_ptr (list_eventval_to_list_val ge vs))
+          (CROSS: Genv.type_of_call ge (comp_of f) (comp_of fd) = Genv.CrossCompartmentCall)
+          (ALLOW: Genv.allowed_cross_call ge (comp_of f) (Vptr b Ptrofs.zero))
+      :
+        Star (Clight.semantics1 p)
+             (State f (code_of_event ev) k e le m)
+             (ev :: nil)
+             (Callstate fd (list_eventval_to_list_val ge vs) (Kcall None f e le k) m).
+    Proof.
+      subst; simpl. unfold code_of_call.
+      econstructor 2.
+      3:{ rewrite E0_right. reflexivity. }
+      { eapply step_call; simpl; eauto.
+        { eapply eval_Elvalue.
+          - eapply eval_Evar_global; eauto.
+          - eapply deref_loc_reference. auto.
+        }
+        { eapply list_eventval_to_expr_val_eval; auto.
+          eapply Forall_impl. 2: eauto. intros. apply wf_eventval_pub_ge; auto. }
+        red; auto.
+        unfold Genv.find_comp. setoid_rewrite FINDF.
+        eapply call_trace_cross; eauto. apply Genv.find_invert_symbol; auto.
+        eapply (list_eventval_to_expr_val_match (globalenv p)); eauto.
+      }
+      econstructor 1.
+    Qed.
+
+    Lemma code_of_event_step_call_internal
+          p f k e le m
+          ge
+          (GE: ge = globalenv p)
+          (* bt should ensure them *)
+          fd args f1
+          (INTERNAL: fd = Internal f1)
+          (* asm should ensure them *)
+          (* handle during proving *)
+          e1 le1 m1
+          (ENTRY: function_entry1 ge f1 args m e1 le1 m1)
+      :
+        Star (Clight.semantics1 p)
+             (Callstate fd args (Kcall None f e le k) m)
+             nil
+             (State f1 (fn_body f1) (Kcall None f e le k) e1 le1 m1).
+    Proof.
+      subst; simpl.
+      econstructor 2.
+      3:{ rewrite E0_right. reflexivity. }
+      { eapply step_internal_function; eauto. }
+      econstructor 1.
+    Qed.
+
+    Lemma code_of_event_step_call_external
+          p m
+          ge
+          (GE: ge = globalenv p)
+          (* bt should ensure them *)
+          fd k args ef targs tres cconv
+          (EXTERNAL: fd = External ef targs tres cconv)
+          (* asm should ensure them *)
+          sev
+          vres m1
+          (SEM: external_call ef ge (call_comp k) args m (sev :: nil) vres m1)
+          (* handle during proving *)
+          sname sargs svr
+          (SYSEV: sev = Event_syscall sname sargs svr)
+      :
+        Star (Clight.semantics1 p)
+             (Callstate fd args k m)
+             (sev :: nil)
+             (Returnstate vres k m1 (rettype_of_type tres) (comp_of ef)).
+    Proof.
+      subst; simpl.
+      econstructor 2.
+      3:{ rewrite E0_right. reflexivity. }
+      { eapply step_external_function; eauto. }
+      econstructor 1.
+    Qed.
+
+    Lemma code_of_event_step_return
+          ev
+          cp cp' rv
+          p f k e le m
+          ge
+          (GE: ge = globalenv p)
+          (EV: ev = Event_return cp' cp rv)
+          (* bt should ensure them *)
+          (WFRV1: wf_eventval_env e rv)
+          (WFRV2: wf_eventval_pub ge rv)
+          (RTTYP: fn_return f = eventval_to_type rv)
+          (* asm should ensure them *)
+          optid f' e' le' k'
+          (CONT: call_cont k = Kcall optid f' e' le' k')
+          (CP1: cp = comp_of f)
+          (CP2: cp' = comp_of f')
+          (NPTR: not_ptr (eventval_to_val ge rv))
+          (CROSS: Genv.type_of_call ge (comp_of f') (comp_of f) = Genv.CrossCompartmentCall)
+          (* handle during proving *)
+          m'
+          (FREE: Mem.free_list m (blocks_of_env ge e) (comp_of f) = Some m')
+      :
+      Star (Clight.semantics1 p)
+           (State f (code_of_event ev) k e le m)
+           (ev :: nil)
+           (State f' Sskip k' e' (set_opttemp optid (eventval_to_val ge rv) le') m').
+    Proof.
+      subst; simpl. unfold code_of_return.
+      econstructor 2.
+      3:{ rewrite E0_left. reflexivity. }
+      { eapply step_return_1; simpl; eauto.
+        { eapply eventval_to_expr_val_eval; auto. apply wf_eventval_pub_ge; auto. }
+        { rewrite RTTYP. eapply sem_cast_eventval; auto. eapply wf_eventval_pub_ge; eauto. }
+      }
+      econstructor 2.
+      3:{ rewrite E0_right. reflexivity. }
+      { rewrite CONT. eapply step_returnstate; auto.
+        econstructor 2; auto. rewrite RTTYP. eapply eventval_to_expr_val_match; eauto.
+        clear. destruct rv; simpl; auto.
+      }
+      econstructor 1.
+    Qed.
+
+  End WELLFORMED.
 
 
   (* TODO *)
